tests/tactics/success/0000-trivial.ec
@@ -1,4 +1,4 @@
 lemma l: forall x, x <=> x.
 proof.
-trivial.
+smt.
 save.
